add a skip_write, revise the handling of probe init

src/3d/prelude/EverParse3d.ProbeActions.fst
@@ -12,6 +12,11 @@ open LowStar.Buffer
 open LowStar.BufferOps
 open FStar.HyperStack.ST
 
+let live_and_unread (dest:copy_buffer_t) h =
+  let sl = stream_of dest in
+  I.live sl h /\
+  Seq.length (I.get_read sl h) == 0
+
 let probe_fn = src:U64.t -> len:U64.t -> dest:copy_buffer_t ->
   Stack bool
     (fun h0 ->
@@ -36,11 +41,10 @@ let probe_fn_incremental =
   dest:copy_buffer_t ->
   Stack bool
     (fun h0 ->
-      I.live (stream_of dest) h0)
+      live_and_unread dest h0)
     (fun h0 b h1 ->
       let sl = stream_of dest in
-      I.live sl h1 /\
-      Seq.length (I.get_read sl h1) == 0 /\
+      live_and_unread dest h1 /\
       (if b
        then (
         UInt.fits (U64.v read_offset + U64.v bytes_to_read) 64 /\
@@ -60,9 +64,8 @@ let init_probe_dest_t =
       I.live (stream_of dest) h0)
     (fun h0 b h1 ->
       let sl = stream_of dest in
-      I.live sl h1 /\
-      modifies (I.footprint sl) h0 h1 /\
-      Seq.length (I.get_read sl h1) == Seq.length (I.get_read sl h0))
+      live_and_unread dest h1 /\
+      modifies (I.footprint sl) h0 h1)
 
 inline_for_extraction
 let write_at_offset_t (t:Type0) (n:U64.t) =
@@ -71,11 +74,10 @@ let write_at_offset_t (t:Type0) (n:U64.t) =
   dest:copy_buffer_t ->
   Stack bool
     (fun h0 ->
-      I.live (stream_of dest) h0)
+      live_and_unread dest h0)
     (fun h0 b h1 ->
       let sl = stream_of dest in
-      I.live sl h1 /\
-      Seq.length (I.get_read sl h1) == 0 /\
+      live_and_unread dest h1 /\
       (if b
        then (
         UInt.fits (U64.v write_offset + U64.v n) 64 /\
@@ -96,11 +98,12 @@ let probe_and_read_at_offset_t (t:Type0) (size_t:U64.t) =
   dest:copy_buffer_t ->
   Stack t
     (fun h0 ->
+      let sl = stream_of dest in
       B.live h0 failed /\
       B.get h0 failed 0 == false /\
-      I.live (stream_of dest) h0)
+      live_and_unread dest h0)
     (fun h0 _ h1 ->
-      I.live (stream_of dest) h1 /\
+      live_and_unread dest h1 /\
       B.live h1 failed /\ 
       B.modifies (B.loc_buffer failed) h0 h1 /\ (
         let has_failed = B.get h1 failed 0 in
@@ -125,7 +128,7 @@ inline_for_extraction
 type probe_m_result a = a
 
 inline_for_extraction
-let probe_m a =
+let probe_m a (requires_unread_dest:bool) =
   read_offset:B.pointer U64.t ->
   write_offset:B.pointer U64.t ->
   failed:B.pointer bool ->
@@ -133,6 +136,7 @@ let probe_m a =
   dest:copy_buffer_t ->
   Stack (probe_m_result a)
     (fun h0 ->
+      let sl = stream_of dest in
       B.live h0 read_offset /\
       B.live h0 write_offset /\
       B.live h0 failed /\
@@ -147,10 +151,11 @@ let probe_m a =
             (B.loc_buffer write_offset)))
         (loc_of dest) /\
       B.get h0 failed 0 == false /\
-      I.live (stream_of dest) h0)
+      I.live sl h0 /\
+      (requires_unread_dest ==> Seq.length (I.get_read sl h0) == 0))
     (fun h0 res h1 ->
       let sl = stream_of dest in
-      I.live sl h1 /\
+      live_and_unread dest h1 /\
       B.live h1 read_offset /\
       B.live h1 write_offset /\
       B.live h1 failed /\
@@ -162,8 +167,6 @@ let probe_m a =
         let has_failed = B.get h1 failed 0 in
         U64.(w1 >=^ w0) /\
         U64.(r1 >=^ r0) /\
-        (w0=w1 ==> Seq.length (I.get_read sl h1) == Seq.length (I.get_read sl h0)) /\
-        (w0<>w1 ==> Seq.length (I.get_read sl h1) == 0) /\
         modifies 
             (B.loc_union 
               (B.loc_union 
@@ -176,7 +179,7 @@ let probe_m a =
 inline_for_extraction
 noextract
 let probe_fn_incremental_as_probe_m (f:probe_fn_incremental) (bytes_to_read:U64.t { bytes_to_read <> 0uL}) 
-: probe_m unit
+: probe_m unit true
 = fun read_offset write_offset failed src dest ->
     let h0  = get () in
     let rd = !*read_offset in
@@ -195,7 +198,7 @@ let probe_fn_incremental_as_probe_m (f:probe_fn_incremental) (bytes_to_read:U64.
 inline_for_extraction
 noextract
 let init_probe_m (f:init_probe_dest_t) (sz:U64.t)
-: probe_m unit
+: probe_m unit false
 = fun read_offset write_offset failed src dest ->
     let ok = f sz dest in
     if ok
@@ -208,7 +211,7 @@ let init_probe_m (f:init_probe_dest_t) (sz:U64.t)
 inline_for_extraction
 noextract
 let write_at_offset_m (#t:Type0) (#w:U64.t { w <> 0uL }) (f:write_at_offset_t t w) (v:t)
-: probe_m unit
+: probe_m unit true
 = fun read_offset write_offset failed src dest ->
     let wr = !*write_offset in
     let ok = f v wr dest in
@@ -223,7 +226,7 @@ let write_at_offset_m (#t:Type0) (#w:U64.t { w <> 0uL }) (f:write_at_offset_t t 
 inline_for_extraction
 noextract
 let probe_and_read_at_offset_m (#t:Type0) (#s:U64.t { s <> 0uL }) (reader:probe_and_read_at_offset_t t s)
-: probe_m t
+: probe_m t true
 = fun read_offset write_offset failed src dest ->
     let rd = !*read_offset in
     let v = reader failed rd src dest in
@@ -236,8 +239,8 @@ let probe_and_read_at_offset_m (#t:Type0) (#s:U64.t { s <> 0uL }) (reader:probe_
 
 inline_for_extraction
 noextract
-let seq_probe_m (#a:Type) (dflt:a) (m1:probe_m unit) (m2:probe_m a)
-: probe_m a
+let seq_probe_m (#a:Type) (#req #req':bool) (dflt:a) (m1:probe_m unit req) (m2:probe_m a req')
+: probe_m a req
 = fun read_offset write_offset failed src dest ->
     let res1 = m1 read_offset write_offset failed src dest in
     let has_failed = !*failed in
@@ -247,8 +250,8 @@ let seq_probe_m (#a:Type) (dflt:a) (m1:probe_m unit) (m2:probe_m a)
 
 inline_for_extraction
 noextract
-let bind_probe_m (#a #b:Type) (dflt:b) (m1:probe_m a) (m2:a -> probe_m b)
-: probe_m b
+let bind_probe_m (#a #b:Type) (#req #req':bool) (dflt:b) (m1:probe_m a req) (m2:a -> probe_m b req')
+: probe_m b req
 = fun read_offset write_offset failed src dest ->
     let res1 = m1 read_offset write_offset failed src dest in
     let has_failed = !*failed in
@@ -258,7 +261,7 @@ let bind_probe_m (#a #b:Type) (dflt:b) (m1:probe_m a) (m2:a -> probe_m b)
 inline_for_extraction
 noextract
 let return_probe_m (#a:Type) (v:a)
-: probe_m a
+: probe_m a true
 = fun read_offset write_offset failed src dest -> v
 
 inline_for_extraction
@@ -269,8 +272,8 @@ let check_overflow_add (x:U64.t) (y:U64.t)
 
 inline_for_extraction
 noextract
-let skip (bytes_to_skip:U64.t)
-: probe_m unit
+let skip_read (bytes_to_skip:U64.t)
+: probe_m unit true
 = fun read_offset write_offset failed src dest ->
     let rd = !*read_offset in
     if check_overflow_add rd bytes_to_skip
@@ -283,15 +286,29 @@ let skip (bytes_to_skip:U64.t)
 
 inline_for_extraction
 noextract
+let skip_write (bytes_to_skip:U64.t)
+: probe_m unit true
+= fun read_offset write_offset failed src dest ->
+    let wr = !*write_offset in
+    if check_overflow_add wr bytes_to_skip
+    then (
+      write_offset *= U64.(wr +^ bytes_to_skip)
+    )
+    else (
+      failed *= true
+    )  
+
+inline_for_extraction
+noextract
 let fail
-: probe_m unit
+: probe_m unit true
 = fun read_offset write_offset failed src dest ->
     failed *= true
 
 inline_for_extraction
 noextract
-let if_then_else (b:bool) (m0 m1:probe_m unit)
-: probe_m unit
+let if_then_else (#req:bool) (b:bool) (m0 m1:probe_m unit req)
+: probe_m unit req
 = fun read_offset write_offset failed src dest ->
     if b
     then m0 read_offset write_offset failed src dest
@@ -303,25 +320,12 @@ let pure_external_action t =
 inline_for_extraction
 noextract
 let lift_pure_external_action (#a:Type) (f:pure_external_action a)
-: probe_m a
+: probe_m a true
 = fun read_offset write_offset failed src dest -> f()
-
-let probe_read_t0_and_write_t1
-    (t0 t1:Type0)
-    (size_t0:U64.t { size_t0 <> 0uL })
-    (size_t1:U64.t { size_t1 <> 0uL })
-    (reader:probe_and_read_at_offset_t t0 size_t0)
-    (writer:write_at_offset_t t1 size_t1)
-    (coerce_t0_t1:coerce_value_t t0 t1)
-: probe_m unit
-= bind_probe_m ()
-    (probe_and_read_at_offset_m reader)
-    (fun v -> write_at_offset_m writer (coerce_t0_t1 v)) 
-
 
 inline_for_extraction
 let probe_fn_as_probe_m (bytes_to_read:U64.t) (f:probe_fn)
-: probe_m unit
+: probe_m unit true
 = fun read_offset write_offset failed src dest ->
     let rd = !*read_offset in
     let wr = !*write_offset in
@@ -348,7 +352,7 @@ let probe_fn_as_probe_m (bytes_to_read:U64.t) (f:probe_fn)
 
 inline_for_extraction
 noextract
-let run_probe_m (m:probe_m unit) (src:U64.t) (dest:copy_buffer_t)
+let run_probe_m (m:probe_m unit false) (src:U64.t) (dest:copy_buffer_t)
 : Stack U64.t
     (fun h0 ->
       let sl = stream_of dest in
